Ported revisions 5660:5688 from HOL to HOL-Omega.
Also revised instructions on porting and merging such revisions into HOL-Omega.

examples/ARM/v4T/arm_evalLib.sig
@@ -4,6 +4,7 @@ sig
 
    type mode
    type sys_state
+   type sys_state3
 
    val arm_compset          : computeLib.compset
    val ARM_CONV             : conv
@@ -22,25 +23,37 @@ sig
    val set_registers        : term -> term frag list -> term
    val set_status_registers : term -> term frag list -> term
 
-   val dest_state           : term -> sys_state
-   val mk_state             : sys_state -> term
+   val print_all_regs       : term -> unit
+   val print_usr_regs       : term -> unit
+   val print_std_regs       : term -> unit
+   val print_regs           : (int * mode) list -> term -> unit
+   val print_mem_range      : term -> Arbnum.num * int -> unit
+   val print_mem_block      : term -> int -> unit
 
-   val print_all_regs   : term -> unit
-   val print_usr_regs   : term -> unit
-   val print_std_regs   : term -> unit
-   val print_regs       : (int * mode) list -> term -> unit
-   val print_mem_range  : term -> Arbnum.num * int -> unit
-   val print_mem_block  : term -> int -> unit
+   val load_mem     : string -> int -> Arbnum.num -> term -> term
+   val save_mem     : string -> Arbnum.num -> Arbnum.num -> bool -> term -> unit
 
-   val load_mem    : string -> int -> Arbnum.num -> term -> term
-   val save_mem    : string -> Arbnum.num -> Arbnum.num -> bool -> term -> unit
+   val dest_state   : term -> sys_state
+   val mk_state     : sys_state -> term
 
-   val init        : term * term * term * term -> sys_state -> thm
-   val next        : (term * term * term * term) -> thm -> thm
+   val init         : term * term * term * term -> sys_state -> thm
+   val next         : (term * term * term * term) -> thm -> thm
 
-   val eval_cp     : int * (term * term * term * term) * sys_state -> thm list
-   val evaluate_cp : int * (term * term * term * term) * sys_state -> thm
+   val eval_cp      : int * (term * term * term * term) * sys_state -> thm list
+   val evaluate_cp  : int * (term * term * term * term) * sys_state -> thm
 
-   val eval        : int * term * term * term -> thm list
-   val evaluate    : int * term * term * term -> thm
+   val eval         : int * term * term * term -> thm list
+   val evaluate     : int * term * term * term -> thm
+
+   val dest_state3  : term -> sys_state3
+   val mk_state3    : sys_state3 -> term
+
+   val init3        : term * term * term * term -> sys_state3 -> thm
+   val next3        : (term * term * term * term) -> thm -> thm
+
+   val eval_cp3     : int * (term * term * term * term) * sys_state3 -> thm list
+   val evaluate_cp3 : int * (term * term * term * term) * sys_state3 -> thm
+
+   val eval3        : int * term * term * term -> thm list
+   val evaluate3    : int * term * term * term -> thm
 end
